src/sys_verif/program_proof/demos/stack_proof.v
@@ -19,7 +19,9 @@ From sys_verif.program_proof Require Import prelude empty_ffi.
 From sys_verif.program_proof Require Import heap_init.
 
 Section proof.
-Context `{hG: !heapGS Σ} `{!globalsGS Σ} {go_ctx: GoContext}.
+Context `{hG: !heapGS Σ} {sem : go.Semantics} {package_sem : heap.Assumptions}.
+Collection W := sem + package_sem.
+Set Default Proof Using "W".
 
 (*| The stack representation invariant has one interesting detail: when we
 "push" to the stack it will go from `stack_rep l xs` to `stack_rep l (cons x
@@ -40,27 +42,29 @@ Definition stack_rep (l: loc) (xs: list w64): iProp Σ :=
     "elements" ∷ l.[heap.Stack.t, "elements"] ↦ s ∗
     (* The code appends because this is both easier and more efficient, thus the
     code elements are reversed compared to the abstract state. *)
-    "Hels" ∷ own_slice s (DfracOwn 1) (reverse xs) ∗
+    "Hels" ∷ s ↦* (reverse xs) ∗
     "Hels_cap" ∷ own_slice_cap w64 s (DfracOwn 1).
 
 Lemma wp_NewStack :
-  {{{ is_pkg_init heap.heap }}}
+  {{{ is_pkg_init heap }}}
     @! heap.heap.NewStack #()
   {{{ l, RET #l; stack_rep l [] }}}.
 Proof.
   wp_start as "_".
+  wp_apply wp_slice_literal as "% _".
+  { iIntros. wp_auto. iFrame. }
   wp_alloc l as "H".
   wp_auto.
-  iApply struct_fields_split in "H". iNamed "H". cbn [heap.Stack.elements'].
-  wp_finish.
+  iStructNamed "H". simpl.
+  wp_end.
   iFrame.
   iSplitL.
-  - iApply own_slice_nil.
-  - iApply own_slice_cap_nil.
+  - iApply own_slice_empty; done.
+  - iApply own_slice_cap_empty; done.
 Qed.
 
 Lemma wp_Stack__Push l xs (x: w64) :
-  {{{ is_pkg_init heap.heap ∗ stack_rep l xs }}}
+  {{{ is_pkg_init heap ∗ stack_rep l xs }}}
     l @! (go.PointerType heap.Stack) @! "Push" #x
   {{{ RET #(); stack_rep l (x :: xs) }}}.
 Proof.
@@ -68,10 +72,11 @@ Proof.
   iNamed "Hstack".
   wp_auto.
   wp_apply (wp_slice_literal) as "%s_tmp Hs_tmp".
+  { iIntros. wp_auto. iFrame. }
   wp_apply (wp_slice_append with "[$Hels $Hels_cap $Hs_tmp]").
   iIntros (s') "(Hels & Hels_cap & Hs_tmp)".
   wp_auto.
-  wp_finish.
+  wp_end.
   iFrame "elements Hels_cap".
   rewrite reverse_cons.
   iFrame.
@@ -99,7 +104,7 @@ Qed.
 Hint Rewrite @length_reverse : len.
 
 Lemma wp_Stack__Pop l xs :
-  {{{ is_pkg_init heap.heap ∗ stack_rep l xs }}}
+  {{{ is_pkg_init heap ∗ stack_rep l xs }}}
     l @! (go.PointerType heap.Stack) @! "Pop" #()
   {{{ (x: w64) (ok: bool) xs', RET (#x, #ok);
       stack_rep l xs' ∗
@@ -111,7 +116,7 @@ Proof.
   iDestruct (own_slice_len with "Hels") as %Hlen.
   wp_if_destruct.
   {
-    wp_finish.
+    wp_end.
     iFrame.
     iPureIntro.
     rewrite /stack_pop.
@@ -124,46 +129,44 @@ Proof.
   }
   assert (0 < length xs).
   { rewrite length_reverse in Hlen. word. }
-  wp_pure.
+  rewrite -> decide_True by word.
+  list_elem (reverse xs) (sint.nat (slice.len s) - 1)%nat as x_last.
   { word. }
-  list_elem (reverse xs) (sint.nat (slice.len_f s) - 1)%nat as x_last.
+  wp_apply (wp_load_slice_index with "[$Hels]").
   { word. }
-  wp_apply (wp_load_slice_elem with "[$Hels]").
-  { word. }
-  { replace (sint.nat (word.sub (slice.len_f s) (W64 1))) with (sint.nat (slice.len_f s) - 1)%nat by word.
+  { replace (sint.nat (word.sub (slice.len s) (W64 1))) with (sint.nat (slice.len s) - 1)%nat by word.
     eauto. }
   iIntros "Hels".
   wp_auto.
   iDestruct (own_slice_wf with "Hels") as %Hcap.
-  wp_pure.
-  { word. }
+  rewrite -> decide_True by word.
   wp_auto.
 
   (* NOTE: need to do this work before iApply due to issue with creating xs'
   evar too early *)
   rewrite length_reverse /= in Hlen.
   apply reverse_lookup_Some in Hx_last_lookup as [Hget ?].
-  replace (length xs - S (sint.nat (slice.len_f s) - 1))%nat with 0%nat
+  replace (length xs - S (sint.nat (slice.len s) - 1))%nat with 0%nat
     in Hget by len.
   destruct xs as [|x0 xs'].
   { exfalso; simpl in *; lia. }
   simpl in Hget.
   assert (x0 = x_last) by congruence. subst.
 
-  wp_finish.
+  wp_end.
   rewrite /stack_rep.
   iFrame "elements".
   iSplit; [ | iPureIntro; reflexivity ].
   rewrite /named.
   simpl in *. (* for length (x :: xs) *)
-  iApply own_slice_trivial_slice_f in "Hels".
-  iDestruct (own_slice_split (word.sub (slice.len_f s) (W64 1)) with "Hels") as "[Hfirst Hrest]".
+  iApply own_slice_trivial_slice in "Hels".
+  iDestruct (own_slice_split (word.sub (slice.len s) (W64 1)) with "Hels") as "[Hfirst Hrest]".
   { word. }
   iDestruct (own_slice_slice_absorb_capacity with "[$Hrest $Hels_cap]") as "$".
   { word. }
   iExactEq "Hfirst".
   repeat f_equal.
-  replace (sint.nat (word.sub (slice.len_f s) (W64 1)) - sint.nat (W64 0))%nat
+  replace (sint.nat (word.sub (slice.len s) (W64 1)) - sint.nat (W64 0))%nat
     with (length xs') by len.
   rewrite reverse_cons.
   rewrite take_app_le; [ len | ].
