src/sys_verif/program_proof/concurrent_init.v
@@ -6,7 +6,7 @@ From Perennial Require Import base.
 
 Section proof.
 Context `{hG: heapGS Σ} `{!ffi_semantics _ _}.
-Context `{!globalsGS Σ} {go_ctx: GoContext}.
+Context {sem : go.Semantics} {package_sem : concurrent.Assumptions}.
 
 #[global] Instance : IsPkgInit (iProp Σ) concurrent := define_is_pkg_init True%I.
 #[global] Instance : GetIsPkgInitWf (iProp Σ) concurrent := build_get_is_pkg_init_wf.
