src/sys_verif/program_proof/demos/fibonacci_proof.v
@@ -26,7 +26,7 @@ From sys_verif.program_proof Require Import functional_init.
 
 Section proof.
 Context `{hG: !heapGS Σ}.
-Context `{!globalsGS Σ} {go_ctx: GoContext}.
+Context {sem : go.Semantics} {package_sem : FILLME.Assumptions}.
 
 Fixpoint fibonacci (n: nat): nat :=
   match n with
