src/sys_verif/program_proof/heap_proof/heap_examples.v
@@ -2,7 +2,7 @@ From sys_verif.program_proof Require Import prelude empty_ffi.
 From sys_verif.program_proof Require Import heap_init.
 
 Section proof.
-Context `{hG: !heapGS Σ} `{!globalsGS Σ} {go_ctx: GoContext}.
+Context `{hG: !heapGS Σ} {sem : go.Semantics} {package_sem : FILLME.Assumptions}.
 
 Lemma wp_Swap (l1 l2: loc) (x y: w64) :
   {{{ is_pkg_init heap.heap ∗ l1 ↦ x ∗ l2 ↦ y }}}
